Leansubst/Basic.lean
@@ -7,38 +7,31 @@ import Leansubst.Defs
 
 namespace Leansubst.Subst'
 
-section
-
 variable {σ : Type}
+
+local notation:arg "⟦" a "⟧" => Quotient.mk (Subst'.setoid σ) a
+
 variable (s t u : Subst' σ)
 variable (i j k : Nat) (x : σ)
 variable (e : Expr σ) (es : List (Expr σ))
 
-local notation:arg "⟦" a "⟧" => Quotient.mk (Subst'.setoid σ) a
+/-- Extensionally equal substitutions have the same effect. -/
+theorem eqv_apply : s ≈ t → s e = t e := by
+  intros h
+  rw [Subst.apply.respects s t h]
 
+/-- Auxiliary function. -/
 def up : Nat → Subst' σ → Subst' σ
   | 0,     s => s
   | i + 1, s => cons (.var 0) (comp (up i s) (shift 1))
 
-theorem get_up_low (h : k < j) : (up j (@shift σ i)).get k = .var k := by
-  induction j generalizing k with
-  | zero => intros; contradiction
-  | succ j ih =>
-    cases Nat.eq_or_lt_of_le (Nat.le_of_lt_succ h) with
-    | inl h' =>
-      subst h'; rw [up]
-      cases k with
-      | zero => rfl
-      | succ k => rw [get, comp_def, ih k (Nat.lt_succ_self _), apply]
-    | inr h' =>
-      rw [up]
-      cases k with
-      | zero => rfl
-      | succ k =>
-        specialize ih _ (Nat.le_of_lt_succ h)
-        rw [get, comp_def, ih, apply]
+/-- Auxiliary function. -/
+def drop : Nat → Subst' σ → Subst' σ
+  | 0,     s => s
+  | i + 1, s => comp (shift 1) (drop i s)
 
-theorem get_up_high (h : j ≤ k) : (up j (@shift σ i)).get k = .var (k + i) := by
+/-- Accessing higher entries of `up shift`. -/
+theorem up_shift_get_high (h : j ≤ k) : (up j (@shift σ i)).get k = .var (k + i) := by
   have ⟨d, hd⟩ := Nat.le.dest h; clear h
   induction j generalizing k d with
   | zero => rfl
@@ -49,80 +42,205 @@ theorem get_up_high (h : j ≤ k) : (up j (@shift σ i)).get k = .var (k + i) :=
     | succ k =>
       rw [get, comp_def]
       rw [Nat.succ_add] at hd; injection hd with hd
-      rw [ih _ _ hd, apply, Nat.succ_add]
+      rw [ih _ _ hd, apply, get, Nat.succ_add]
 
-theorem comp_eqv_comps_special : comp (up j (shift i)) (shift 1) ≈ (comps (up j (shift i)) 1 : Subst' σ) := by
+/-- Accessing lower entries of `up`. -/
+theorem up_get_low (h : k < j) : (up j s).get k = .var k := by
+  induction j generalizing k with
+  | zero => intros; contradiction
+  | succ j ih =>
+    cases Nat.eq_or_lt_of_le (Nat.le_of_lt_succ h) with
+    | inl h' =>
+      subst h'; rw [up]
+      cases k with
+      | zero => rfl
+      | succ k => rw [get, comp_def, ih k (Nat.lt_succ_self _), apply, get]
+    | inr h' =>
+      rw [up]
+      cases k with
+      | zero => rfl
+      | succ k =>
+        specialize ih _ (Nat.le_of_lt_succ h)
+        rw [get, comp_def, ih, apply, get]
+
+/-- Lemma: `applys` agrees with `apply up shift` on variables. -/
+theorem applys_var : applys j i (.var k) = apply (up j (@shift σ i)) (.var k) := by
+  induction j generalizing k with
+  | zero =>
+    rw [up, applys]
+    split
+    case inl _ => rw [apply, get]
+    case inr h => exact (h (Nat.zero_le _)).elim
+  | succ j ih =>
+    simp only [up, apply, applys] at *
+    cases k with
+    | zero => (split <;> try contradiction); rfl
+    | succ k =>
+      simp only [get, comp_def, ← ih]
+      split <;> rename_i h
+      rotate_right; have h : ¬j ≤ k := fun h' => (h (Nat.succ_le_succ h')).elim
+      rotate_right; have h := Nat.le_of_succ_le_succ h
+      all_goals (split <;> try contradiction)
+      case inl => rw [apply, get, Nat.succ_add]
+      case inr => rw [apply, get]
+
+/-- Lemma: `comps` agrees with `comp shift` for LHS in the form of `up shift`.  -/
+theorem comps_eqv_comp_special : comps (up j (shift i)) 1 ≈ comp (up j (shift i)) (@shift σ 1) := by
   intros k
   rw [comp_def, comps_def]
   cases Nat.lt_sum_ge k j with
   | inl h =>
-    rw [get_up_low _ _ _ h, apply, applys]
+    rw [up_get_low _ _ _ h, apply, applys]
     split
     case inl _ => rfl
     case inr h => exact (h (Nat.zero_le _)).elim
   | inr h =>
-    rw [get_up_high _ _ _ h, apply, applys]
+    rw [up_shift_get_high _ _ _ h, apply, applys]
     split
     case inl _ => rfl
     case inr h => exact (h (Nat.zero_le _)).elim
 
-/-- We have to show that `applys` actually agrees with `apply shift`. -/
+/-- Now we have that `applys` actually agrees with `apply up shift`. -/
 theorem applys_def : applys j i e = apply (up j (shift i)) e := by
   revert j
   -- Induction on `e`.
-  apply @Expr.recOn _
-    (fun e => ∀ j, applys j i e = apply (up j (shift i)) e)
-    (List.foldr (fun e etc => (∀ j, applys j i e = apply (up j (shift i)) e) ∧ etc) True)
-    <;> intros <;> try trivial
-  case var k j =>
-    induction j generalizing k with
-    | zero =>
-      rw [up, applys]
-      split
-      case inl _ => rw [apply]
-      case inr h => exact (h (Nat.zero_le _)).elim
-    | succ j ih =>
-      simp only [up, applys, apply_var] at *
-      cases k with
-      | zero => (split <;> try contradiction); rfl
-      | succ k =>
-        simp only [get, comp_def, ← ih]
-        split <;> rename_i h
-        rotate_right; have h : ¬j ≤ k := fun h' => (h (Nat.succ_le_succ h')).elim
-        rotate_right; have h := Nat.le_of_succ_le_succ h
-        all_goals (split <;> try contradiction)
-        case inl => rw [apply, Nat.succ_add]
-        case inr => rw [apply]
-  case binder e ih j =>
-    rw [applys, apply, ih, up]
-    congr 1
-    have h := comp_eqv_comps_special i j (σ := σ)
-    have h' : (.cons (.var 0) ⟦comp (up j (shift i)) (shift 1)⟧ : Subst σ) e =
-              (.cons (.var 0) ⟦comps (up j (shift i)) 1⟧ : Subst σ) e := by rw [Quotient.sound h]
-    exact h'
-  case node x es ih j =>
+  let motive := fun (e : Expr σ) => ∀ j, applys j i e = apply (up j (shift i)) e
+  apply @Expr.recOn _ (fun e => motive e) (List.foldr (fun e etc => motive e ∧ etc) True)
+    <;> intros <;> (try trivial) <;> intros j
+  case var k => exact applys_var _ _ _
+  case binder e ih =>
+    rw [applys, apply, ih, up, eqv_apply]
+    intros k
+    cases k with
+    | zero => rfl
+    | succ => rw [get, get, comps_eqv_comp_special]
+  case node x es ih =>
     induction es with
     | nil => rw [applys, apply, apply.nested]; rfl
     | cons h' t' ih' =>
       rw [List.foldr] at ih
       rw [applys, applys.nested, apply, apply.nested]
-      congr
+      congr 2
       . exact ih.left _
       . specialize ih' ih.right
         rw [applys, apply] at ih'
         injection ih'
 
-theorem apply_apply : t (s e) = (comp s t) e := by
-  sorry
+/-- Now we have that `comps` actually agrees with `comp shift`. -/
+theorem comps_eqv_comp : comps s i ≈ comp s (shift i) := by
+  intros k
+  rw [comp_def, comps_def, applys_def, up]
 
+/-- Applying the identity substitution. -/
 theorem id_apply : (id σ) e = e := by
-  sorry
+  -- Induction on `e`.
+  apply @Expr.recOn _ (fun e => (id σ) e = e) (List.foldr (fun e etc => (id σ) e = e ∧ etc) True)
+    <;> intros <;> (try trivial)
+  case var i => rw [id, apply]; rfl
+  case binder e ih =>
+    conv => rhs; rw [← ih]
+    rw [id, apply, comps, eqv_apply]
+    intros k
+    cases k <;> rfl
+  case node x es ih =>
+    induction es with
+    | nil => rw [id, apply, apply.nested]
+    | cons h' t' ih' =>
+      rw [List.foldr] at ih
+      rw [apply, apply.nested]
+      congr 2
+      . exact ih.left
+      . specialize ih' ih.right
+        rw [id, apply] at ih'
+        injection ih'
 
-end
+/-- Accessing higher entries of `up`. -/
+theorem up_get_high : (up j s).get (j + k) = apply (shift j) (s.get k) := by
+  induction j generalizing k with
+  | zero => rw [up, Nat.zero_add, ← id, id_apply]
+  | succ j ih =>
+    rw [up, Nat.succ_add, get, comp_def, ih]
+    sorry
+
+theorem up_apply_up_shift_apply : (up (i + 1) s) ((up i (shift 1)) e) = (up i (shift 1)) ((up i s) e) := by
+  revert s
+  -- Induction on `e`.
+  let motive := fun (e : Expr σ) => ∀ i s, (up (i + 1) s) ((up i (shift 1)) e) = (up i (shift 1)) ((up i s) e)
+  apply @Expr.recOn _ (fun e => motive e) (List.foldr (fun e etc => motive e ∧ etc) True)
+    <;> intros <;> (try trivial) <;> intros i s
+  case var j =>
+    simp only [get, apply, comp_def]
+    cases Nat.lt_sum_ge j i with
+    | inl h => have h' := Nat.lt_succ_of_lt h; simp only [up_get_low _ _ _ h, up_get_low _ _ _ h', apply]
+    | inr h =>
+      have ⟨d, hd⟩ := Nat.le.dest h; subst hd; clear h
+      simp only [up_get_high _ _ _]
+      rw [get, apply, get, apply, Nat.add_assoc, Nat.add_comm 1 i, Nat.add_comm d (i + 1), up_get_high]
+      sorry
+  case binder e ih =>
+    simp only [apply]
+    congr 1
+    have h : ∀ (t : Subst' σ), cons (Expr.var 0) (comps t 1) ≈ cons (Expr.var 0) (comp t (shift 1)) := by
+      intros t k
+      cases k with
+      | zero => rfl
+      | succ => rw [get]; exact comps_eqv_comp _ _ _
+    simp only [eqv_apply _ _ _ (h _)]; clear h
+    exact ih _ _
+  case node x es ih =>
+    induction es with
+    | nil => simp only [apply, apply.nested] 
+    | cons h' t' ih' =>
+      rw [List.foldr] at ih
+      simp only [apply, apply.nested]
+      congr 2
+      . exact ih.left _ _
+      . specialize ih' ih.right
+        simp only [apply] at ih'
+        injection ih'
+
+/-- Applying composition of substitutions. -/
+theorem apply_apply : t (s e) = (comp s t) e := by
+  -- Induction on `e`.
+  let motive := fun (e : Expr σ) => ∀ t s, t (s e) = (comp s t) e
+  apply @Expr.recOn _ (fun e => motive e) (List.foldr (fun e etc => (motive e) ∧ etc) True)
+    <;> intros <;> (try trivial) <;> intros t s
+  case var i => simp only [comp_def, apply]
+  case binder e ih =>
+    simp only [apply]
+    rw [ih, eqv_apply]
+    intros k
+    cases k with
+    | zero => simp only [get, comp_def, apply]
+    | succ k =>
+      simp only [get, comp_def, comps_def, applys_def, up]
+      have h : cons (Expr.var 0) (comps t 1) ≈ cons (Expr.var 0) (comp t (shift 1)) := by
+        intros k
+        cases k with
+        | zero => rfl
+        | succ => rw [get]; exact comps_eqv_comp _ _ _
+      rw [eqv_apply _ _ _ h]; clear h
+      exact up_apply_up_shift_apply _ 0 _
+  case node x es ih =>
+    -- TODO: make a tactic to solve this case...
+    induction es with
+    | nil => simp only [apply, apply.nested] 
+    | cons h' t' ih' =>
+      rw [List.foldr] at ih
+      simp only [apply, apply.nested]
+      congr 2
+      . exact ih.left _ _
+      . specialize ih' ih.right
+        simp only [apply] at ih'
+        injection ih'
 
 end Subst'
 
 namespace Subst
+
+variable {σ : Type}
+
+local notation:arg "⟦" a "⟧" => Quotient.mk (Subst'.setoid σ) a
 
 @[simp] theorem shift_wrap (n : Nat) : ⟦Subst'.shift n⟧ = Subst.shift σ n := rfl
 @[simp] theorem cons_wrap (e : Expr σ) (s : Subst' σ) : ⟦Subst'.cons e s⟧ = Subst.cons e ⟦s⟧ := rfl
@@ -133,51 +251,41 @@ namespace Subst
 @[simp] theorem comps_wrap (s : Subst' σ) (n : Nat) : ⟦Subst'.comps s n⟧ = Subst.comps ⟦s⟧ n := rfl
 @[simp] theorem comp_wrap (s t : Subst' σ) : ⟦Subst'.comp s t⟧ = Subst.comp ⟦s⟧ ⟦t⟧ := rfl
 
-section
-
-variable {σ : Type}
 variable (s t u : Subst σ)
 variable (i j k : Nat) (x : σ)
 variable (e : Expr σ) (es : List (Expr σ))
 
-local notation:arg "⟦" a "⟧" => Quotient.mk (Subst'.setoid σ) a
-
 @[simp]
 theorem get_zero : (cons e s).get 0 = e := by
   induction s using Quotient.ind
-  rw [← cons_wrap, ← get_wrap]
-  rfl
+  rw [← cons_wrap, ← get_wrap]; rfl
 
 @[simp]
 theorem get_succ : (cons e s).get (i + 1) = s.get i := by
   induction s using Quotient.ind
-  rw [← cons_wrap, ← get_wrap]
-  rfl
+  rw [← cons_wrap, ← get_wrap]; rfl
 
 @[simp]
-theorem shift_zero : shift σ 0 = id σ := by
-  rfl
+theorem shift_zero : shift σ 0 = id σ := rfl
 
 @[simp]
 theorem shift_succ_succ : shift σ (i + 1 + 1) = comp (shift σ (i + 1)) (shift σ 1) := by
   simp only [← shift_wrap, ← comp_wrap]
   apply Quotient.sound
-  intros j
-  rfl
+  intros k; rfl
 
 @[simp]
 theorem comps_expand : comps s i = comp s (shift σ i) := by
   induction s using Quotient.ind
   rw [← comps_wrap, ← shift_wrap, ← comp_wrap]
   apply Quotient.sound
-  intros j
-  rw [Subst'.comps_def, Subst'.comp_def, Subst'.applys_def]
-  rfl
+  intros k
+  rw [Subst'.comps_def, Subst'.comp_def, Subst'.applys_def]; rfl
 
 @[simp]
 theorem apply_var : s (.var i) = s.get i := by
   induction s using Quotient.ind
-  rw [← apply_wrap, ← get_wrap, Subst'.apply_var]
+  rw [← apply_wrap, ← get_wrap, Subst'.apply]
 
 @[simp]
 theorem apply_binder : s (.binder e) = .binder ((cons (.var 0) (comp s (shift σ 1))) e) := by
@@ -213,16 +321,15 @@ theorem id_comp : comp (id σ) s = s := by
   induction s using Quotient.ind
   rw [← id_wrap, ← comp_wrap]
   apply Quotient.sound
-  intros j
-  rw [Subst'.id, Subst'.comp_def, Subst'.get, Subst'.apply_var]
-  rfl
+  intros k
+  rw [Subst'.id, Subst'.comp_def, Subst'.get, Subst'.apply]; rfl
 
 @[simp]
 theorem comp_id : comp s (id σ) = s := by
   induction s using Quotient.ind; rename_i s
   rw [← id_wrap, ← comp_wrap]
   apply Quotient.sound
-  intros j
+  intros k
   rw [Subst'.comp_def, apply_wrap, id_wrap, id_apply]
 
 @[simp]
@@ -230,8 +337,8 @@ theorem shift_comp_cons : comp (shift σ 1) (cons e s) = s := by
   induction s using Quotient.ind; rename_i s
   rw [← cons_wrap, ← shift_wrap, ← comp_wrap]
   apply Quotient.sound
-  intros j
-  rw [Subst'.comp_def, Subst'.get, Subst'.apply, Subst'.apply_var]
+  intros k
+  rw [Subst'.comp_def, Subst'.get, Subst'.apply, Subst'.get]
 
 @[simp]
 theorem cons_comp : comp (cons e s) t = cons (t e) (comp s t) := by
@@ -239,10 +346,10 @@ theorem cons_comp : comp (cons e s) t = cons (t e) (comp s t) := by
   induction t using Quotient.ind; rename_i t
   simp only [← apply_wrap, ← cons_wrap, ← comp_wrap]
   apply Quotient.sound
-  intros j
-  cases j with
+  intros k
+  cases k with
   | zero => rw [Subst'.comp_def, Subst'.get]; rfl
-  | succ j => rw [Subst'.comp_def, Subst'.get, Subst'.get, Subst'.comp_def]
+  | succ => rw [Subst'.comp_def, Subst'.get, Subst'.get, Subst'.comp_def]
 
 @[simp]
 theorem comp_assoc : comp (comp s t) u = comp s (comp t u) := by
@@ -251,34 +358,29 @@ theorem comp_assoc : comp (comp s t) u = comp s (comp t u) := by
   induction u using Quotient.ind; rename_i u
   simp only [← comp_wrap]
   apply Quotient.sound
-  intros j
+  intros k
   simp only [Subst'.comp_def, Subst'.apply]
   simp only [get_wrap, apply_wrap, apply_apply, comp_wrap]
 
 @[simp]
 theorem apply_zero_cons_shift_comp : cons (s (.var 0)) (comp (shift σ 1) s) = s := by
   induction s using Quotient.ind; rename_i s
-  rw [← apply_wrap, Subst'.apply_var, ← shift_wrap, ← comp_wrap, ← cons_wrap]
+  rw [← apply_wrap, Subst'.apply, ← shift_wrap, ← comp_wrap, ← cons_wrap]
   apply Quotient.sound
-  intros j
-  cases j with
+  intros k
+  cases k with
   | zero => rfl
-  | succ j => rw [Subst'.get, Subst'.comp_def, Subst'.get, Subst'.apply_var]
+  | succ => rw [Subst'.get, Subst'.comp_def, Subst'.get, Subst'.apply]
 
 @[simp]
 theorem zero_cons_shift : cons (.var 0) (shift σ 1) = id σ := by
   rw [← shift_wrap, ← id_wrap, ← cons_wrap]
   apply Quotient.sound
-  intros j
-  cases j with
-  | zero => rfl
-  | succ => rfl
+  intros k; cases k <;> rfl
 
 /-
 example : comp (shift σ 1) (id σ) = shift σ 1 := by
   simp
 -/
-
-end
 
 end Leansubst.Subst
