Leansubst/Examples.lean
@@ -1,3 +1,3 @@
 import Leansubst.Basic
 
-def hello := "world"
+
